src/escjava/trunk/MobiusDirectVCGen/src/mobius/directVCGen/formula/Lookup.java
@@ -1,36 +1,98 @@
 package mobius.directVCGen.formula;
 
+import java.util.Vector;
+
 import mobius.directVCGen.vcgen.struct.Post;
 
+import escjava.ast.Modifiers;
+import escjava.ast.TagConstants;
 import escjava.sortedProver.Lifter.Term;
+import escjava.sortedProver.NodeBuilder.FnSymbol;
+import escjava.sortedProver.NodeBuilder.Sort;
 import javafe.ast.ClassDecl;
+import javafe.ast.ConstructorDecl;
+import javafe.ast.FormalParaDecl;
+import javafe.ast.FormalParaDeclVec;
 import javafe.ast.MethodDecl;
+import javafe.ast.RoutineDecl;
 
 public class Lookup {
+	public static Vector<FnSymbol> symToDeclare = new Vector<FnSymbol>();
 
+	public static Term buildStdCond (RoutineDecl m, String name, boolean hasResult) {
+		int arity = m.args.size();
+		boolean incThis = false;
+		
+		Sort returnType = Ref.sort;  
+		if(m instanceof MethodDecl) {
+			returnType = Type.typeToSort(((MethodDecl) m).returnType);
+		}
+		if((m.getModifiers() & Modifiers.ACC_STATIC) == 0) {
+			arity ++;
+			incThis = true;
+		}
+		if((m instanceof ConstructorDecl) ||
+				((MethodDecl)m).returnType.getTag() == TagConstants.VOIDTYPE) {
+			hasResult = false;
+		}
+		if(hasResult) {
+			arity++;
+		}
+		Sort [] s = new Sort[arity];
+		Term [] args = new Term [arity];
+		if(incThis) {
+			s [0] = Ref.sort;
+			args[0] = Ref.varthis;
+		}
+		FormalParaDeclVec v = m.args;
+		for(int i = 0; i < v.size(); i ++) {
+			FormalParaDecl para = v.elementAt(i);
+			args[i + 1] = Expression.rvar(para);
+			s[i + 1] = args[i+1].getSort();
+			
+		}
+		if(hasResult) {
+			args[args.length - 1] = Expression.rvar(Expression.result, returnType);
+			s[s.length - 1] = args[args.length - 1].getSort();
+		}
+		if(m instanceof ConstructorDecl) {
+			name = ((ConstructorDecl)m).parent + name;
+		}
+		else {
+			name = ((MethodDecl)m).id+ name;
+		}
+		FnSymbol sym = Formula.lf.registerPredSymbol(name, s);
+		symToDeclare.add(sym);
+		
+		return Formula.lf.mkFnTerm(sym, args);
+		
+	}
 	/**
 	 * Returns the FOL Term representation of the precondition of method m.
 	 * @param m the method of interest
 	 */
-	public static Term precondition(MethodDecl m){
-		return Expression.rvar(m.id + "_pre", Logic.sort);//Logic.True();
+	public static Term precondition(RoutineDecl m){
+		
+		return buildStdCond (m, "_pre", false);
 	}
 
 	/**
 	 * Returns the FOL Term representation of the normal postcondition of method m.
 	 * @param m the method of interest
 	 */
-	public static Post normalPostcondition(MethodDecl m){
-		return new Post(Expression.rvar(Formula.lf.sortRef),Expression.rvar(m.id + "_norm", Logic.sort));//Logic.True());
+	public static Post normalPostcondition(RoutineDecl m){
+		return new Post(buildStdCond (m, "_norm", true)); 
 	}
-
+	public static Post normalPostcondition(MethodDecl m){
+		return new Post(Expression.rvar(Expression.result, Type.typeToSort(m.returnType)),buildStdCond (m, "_norm", true)); 
+	}
 	/**
 	 * Returns a vector of   FOL Term representations of the exceptional postconditions of method m.
 	 * The exceptional postcondition will always look like this: Sort => Term
 	 * @param m the method of interest
 	 */
-	public static Post exceptionalPostcondition(MethodDecl m){
-		return new Post(Expression.rvar(Formula.lf.sortRef),Expression.rvar(m.id + "_excp", Logic.sort));//Logic.True());
+	public static Post exceptionalPostcondition(RoutineDecl m){
+		return new Post(Expression.rvar(Expression.result, Ref.sort),buildStdCond (m, "_excp", false)); 
 	}
 
 //	/**
