src/escjava/trunk/MobiusDirectVCGen/src/mobius/directVCGen/formula/coq/CoqFile.java
@@ -4,8 +4,13 @@ import java.io.File;
 import java.io.FileNotFoundException;
 import java.io.FileOutputStream;
 import java.io.PrintStream;
+import java.util.Vector;
 
+import mobius.directVCGen.formula.Formula;
+
+import escjava.sortedProver.NodeBuilder.FnSymbol;
 import escjava.sortedProver.NodeBuilder.STerm;
+import escjava.sortedProver.NodeBuilder.Sort;
 
 public class CoqFile {
 	PrintStream out;
@@ -19,16 +24,6 @@ public class CoqFile {
 	
 	
 	public void writeProof(STerm term) {
-		out.println("Add LoadPath \"" + base + "\".\n" +
-				    "Add LoadPath \"" + base + File.separator + "Formalisation\".\n" +
-		            "Add LoadPath \"" + base + File.separator + "Formalisation" +
-											   File.separator + "Bicolano" + "\".\n" +
-		            "Add LoadPath \"" + base + File.separator + "Formalisation" +
-				   							   File.separator + "Library" + "\".\n" +
-			        "Add LoadPath \"" + base + File.separator + "Formalisation" +
-				   							   File.separator + "Library" + 
-				   							   File.separator + "Map" + "\".\n");
-		out.println("Load \"defs_types.v\".\n");
 		out.println("Lemma l:\n" + term + ".");
 		out.println("Proof.");
 		out.println("intros; repeat (split; intros).\n\nQed.");
@@ -36,6 +31,35 @@ public class CoqFile {
 		
 	public void finalize() {
 		out.close();
+	}
+
+
+	public void writeDefs(Vector<FnSymbol> symToDeclare, Vector<String> classNames) {
+		out.println("Add LoadPath \"" + base + "\".\n" +
+			    "Add LoadPath \"" + base + File.separator + "Formalisation\".\n" +
+	            "Add LoadPath \"" + base + File.separator + "Formalisation" +
+										   File.separator + "Bicolano" + "\".\n" +
+	            "Add LoadPath \"" + base + File.separator + "Formalisation" +
+			   							   File.separator + "Library" + "\".\n" +
+		        "Add LoadPath \"" + base + File.separator + "Formalisation" +
+			   							   File.separator + "Library" + 
+			   							   File.separator + "Map" + "\".\n");
+		out.println("Load \"defs_types.v\".\n");
+		for(String name: classNames) {
+			out.println("Variable " + name + ": ClassName.");
+		}
+		out.println();
+		for(FnSymbol sym : symToDeclare) {
+			out.print("Variable " + sym.name + ": ");
+
+			for(Sort s: sym.argumentTypes) {
+				String str = Formula.getCurrentLifter().builder.buildSort(s).toString();
+				out.print(str + " -> ");
+			}
+			out.println(Formula.getCurrentLifter().builder.buildSort(sym.retType) + ".");
+		}
+		out.println();
+
 	}
 		
 }
