src/escjava/trunk/MobiusDirectVCGen/src/mobius/directVCGen/vcgen/MethodVisitor.java
@@ -10,13 +10,16 @@ import javafe.ast.BlockStmt;
 import javafe.ast.FormalParaDecl;
 import javafe.ast.FormalParaDeclVec;
 import javafe.ast.MethodDecl;
+import mobius.directVCGen.formula.Expression;
 import mobius.directVCGen.formula.Formula;
 import mobius.directVCGen.formula.Logic;
 import mobius.directVCGen.formula.Lookup;
+import mobius.directVCGen.formula.Type;
 import mobius.directVCGen.formula.coq.CoqFile;
 import mobius.directVCGen.vcgen.stmt.StmtVCGen;
 import mobius.directVCGen.vcgen.struct.Post;
 import mobius.directVCGen.vcgen.struct.VCEntry;
+import escjava.sortedProver.Lifter.QuantVariable;
 import escjava.sortedProver.Lifter.Term;
 import escjava.tc.Types;
 
@@ -52,6 +55,7 @@ public class MethodVisitor extends DirectVCGen {
 				fos.println(t);
 				fos.close();
 				CoqFile cf = new CoqFile(configdir, getBaseDir(), name);
+				cf.writeDefs(Lookup.symToDeclare, Type.getAllTypes());
 				cf.writeProof(Formula.generateFormulas(t));
 				
 			}
@@ -84,6 +88,14 @@ public class MethodVisitor extends DirectVCGen {
 		StmtVCGen dvcg = new StmtVCGen();
 		Post pre = (Post)x.accept(dvcg, post);
 		Term po = Logic.implies(Lookup.precondition(meth), pre.post);
+		FormalParaDeclVec vec = meth.args;
+		QuantVariable[] qvs = new QuantVariable[vec.size()];
+		for(int i = 0; i < vec.size(); i++) {
+			FormalParaDecl dec = vec.elementAt(i);
+			QuantVariable qv = Expression.var(dec);
+			qvs[i] = qv;
+		}
+		po = Logic.forall(qvs, po);
 		//System.out.println(po);
 		
 		vcs.add(po);
