src/escjava/trunk/MobiusDirectVCGen/src/mobius/directVCGen/vcgen/expression/ABasicExpressionVCGEn.java
@@ -1,16 +1,16 @@
 package mobius.directVCGen.vcgen.expression;
 
-import escjava.sortedProver.Lifter.QuantVariableRef;
-import escjava.sortedProver.Lifter.Term;
+import javafe.ast.ASTNode;
 import javafe.ast.Expr;
 import mobius.directVCGen.formula.Expression;
 import mobius.directVCGen.formula.Heap;
 import mobius.directVCGen.formula.Logic;
 import mobius.directVCGen.formula.Ref;
-import mobius.directVCGen.formula.Type;
 import mobius.directVCGen.vcgen.stmt.StmtVCGen;
 import mobius.directVCGen.vcgen.struct.Post;
 import mobius.directVCGen.vcgen.struct.VCEntry;
+import escjava.sortedProver.Lifter.QuantVariableRef;
+import escjava.sortedProver.Lifter.Term;
 
 public abstract class ABasicExpressionVCGEn {
 	private ExpressionVisitor visitor;
@@ -20,7 +20,9 @@ public abstract class ABasicExpressionVCGEn {
 	public Post getPre(Expr e, VCEntry post) {
 		return (Post)e.accept(visitor, post);
 	}
-	
+	public Post getPre(ASTNode e, VCEntry post) {
+		return (Post)e.accept(visitor, post);
+	}
 	public Term getNewExcpPost(Term type, VCEntry post) {
 		Post p = StmtVCGen.getExcpPost(type, post);
 		QuantVariableRef e = Expression.rvar(Ref.sort);
